
Appendix B

Distribution-to-Distribution NDT

In this appendix, we start from the approximation of the log-likelihood of pdf addressed in the

Point-to-Distribution NDT [7]. Then, we paraphrase the derivations of the objective function,

the gradient vector, and the Hessian matrix of the Distribution-to-Distribution NDT [6].

Approximation of Log-likelihood of Gaussian Probability Density Function [7]

Let p(x) = N (x | µ, σ2) be the probability density function of a Gaussian distribution.

Minimizing p(x) is often replaced by minimizing log(p(x)) due to the property of logarithms.

However, log(p(x)) could be unbounded below when p(x) is close to zero. To prevent this issue

from happening, Magnusson [7] suggests to add a base pdf value 0 < c2 < 1 and a scale factor

c1 > 0 to approximate p(x), that is,

p(x) =
1

σ
√
2π

exp(−1

2

(x− µ)2

σ2
) (B.1)

≈ p(x) = c1 exp(−
1

2

(x− µ)2

σ2
) + c2. (B.2)

Afterwards, the second approximation is performed to log(p(x))

log(p(x)) = log(c1 exp(−
1

2

(x− µ)2

σ2
) + c2) (B.3)

≈ p̃(x) = d1 exp(−
d2
2

(x− µ)2

σ2
) + d3 (B.4)

where d1, d2 > 0, d3 < 0 are computed by assuming the approximated value and the original

value are identical at µ, µ± σ, and ±∞, that is,

log(p(µ)) = p̃(µ), log(p(µ± σ)) = p̃(µ± σ), log(p(±∞)) = p̃(±∞). (B.5)
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Therefore, we have

d1 = log(c1 + c2)− d3 (B.6)

d2 = −2 log
(
log(c1 exp(−1

2
) + c2)− d3

d1

)
(B.7)

d3 = log(c2). (B.8)

In the implementation in [7], these parameters are chosen as empirical values. Following

the same approximation, we can derive the following multivariate version:

argmax N (x | µ,Σ) = argmax log(N (x | µ,Σ)) (B.9)

≈ argmax d1 exp(−
d2
2
(x− µ)TΣ−1(x− µ)). (B.10)

Note that d3 is omitted since it is a constant and does not influence the optimization.

Objective Function of Distribution-to-Distribution NDT [6]

Recall eq. (3.9), the L2 distance between two NDT models is

DL2(Np,Nq) =

∫
(N (x | µp,Σp)−N (x | µq,Σq))

2 dx

=

∫
(N (x | µp,Σp))

2 dx+

∫
(N (x | µq,Σq))

2 dx

− 2

∫
N (x | µp,Σp) N (x | µq,Σq) dx (B.11)

The first and second terms in eq. (B.11) are constants, and the third term can be simplified as,

− 2

∫
N (x | µp,Σp) N (x | µq,Σq) dx (B.12)

=− 2

∫
N (0 | µp − µq,Σp + Σq) N (x | µc,Σc) dx (B.13)

=− 2 N (0 | µp − µq,Σp + Σq) (B.14)

where µc = (Σ−1
p +Σ−1

q )−1(Σ−1
p µp+Σ−1

q µq), Σc = (Σ−1
p +Σ−1

q )−1. Equation (B.13) follows

eq. (371) in Section 8.1.8 of the Matrix Cookbook [21] and can be proved by expansion.
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After combining all the correspondences, the optimized parameterΘ, and the approximation

in eq. (B.10), the final optimization problem then becomes eq. (3.12).

argmin
Θ

n∏
k=1

DL2(T (Npk,Θ),Nqk) (B.15)

= argmin
R,t

n∏
k=1

DL2(N (Rµpk + t, RΣpkR
T ),N (µqk,Σqk)) (B.16)

= argmin
R,t

−
n∏

k=1

N (0 | Rµpk + t− µqk, RΣpkR
T + Σqk) (B.17)

= argmin
R,t

n∑
k=1

− log(N (0 | Rµpk + t− µqk, RΣpkR
T + Σqk)) (B.18)

≈ argmin
R,t

n∑
k=1

−d1 exp (−
d2
2
(Rµpk + t− µqk)

T (RΣpkR
T + Σqk)

−1(Rµpk + t− µqk))

(B.19)

Gradient Vector and Hessian Matrix of Distribution-to-Distribution NDT [6]

Following the notations in [6], we define

µpq = Rµp + t− µq B = (RΣpR
T + Σq)

−1 (B.20)

ja =
∂µpq

∂Θa

=
∂(Rµp + t)

∂Θa

Za =
∂B−1

∂Θa

=
∂(RΣpR

T )

∂Θa

(B.21)

Hab =
∂2µpq

∂Θa∂Θb

=
∂2(Rµp + t)

∂Θa∂Θb

Zab =
∂2B−1

∂Θa∂Θb

=
∂2(RΣiR

T )

∂Θa∂Θb

(B.22)

The objective function of a single correspondence is

fd2d-ndt(Θ,Np,Nq) = −d1 exp(−
d2
2
µT

pqBµpq) (B.23)

The components of the gradient vector are

∇f(Θ)a =
d1d2
2

exp(−d2
2
µT

pqBµpq) · qa (B.24)

qa = 2µT
pqBja − µT

pqBZaBµpq (B.25)
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Note that we apply the property
∂B

∂Θa

= −B∂B−1

∂Θa

B = −BZaB.

After that, the components of the Hessian matrix are

∇2f(Θ)ab = d1d2 exp(−
d2
2
µT

pqBµpq)(j
T
b Bja − µT

pqBZbBja + µT
pqBHab

−µT
pqBZaBjb + µT

pqBZaBZbBµpq

−1

2
µT

pqBZabBµpq −
d2
4
qaqb). (B.26)

where qb follows eq. (B.25) but use the derivatives to Θb.

Analytical Expressions of ja,Hab, Za, Zab

To compute these expressions, we first compute
∂R

∂Θa

and
∂2R

∂Θa∂Θb

. We have

R = Rx(θx)Ry(θy)Rz(θz) (B.27)

=


cycz −szcy sy

sxsycz + szcx −sxsysz + cxcz −sxcy

sxsz − sycxcz sxcz + syszcx cxcy

 (B.28)

where sx = sin θx, sy = sin θy, sz = sin θz, cx = cos θx, cy = cos θy, cz = cos θz.

The derivatives of R with respect to translation parameters tx, ty, tz are zero matrices since

R is only related to θx, θy, θz, i.e.,

∂R

∂tx
=

∂R

∂ty
=

∂R

∂tz
= 03×3 (B.29)

where 03×3 represents the 3x3 zero matrix.

For the same reason, we have

∂2R

∂Θa∂Θb

= 03×3 (B.30)

where a or b ∈ {tx, ty, tz}.

The next page shows the derivatives of R with respect to θx, θy, θz.
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∂R

∂θx
=


0 0 0

−sxsz + sycxcz −sxcz − syszcx −cxcy

sxsycz + szcx −sxsysz + cxcz −sxcy

 (B.31)

∂R

∂θy
=


−sycz sysz cy

sxcycz −sxszcy sxsy

−cxcycz szcxcy −sycx

 (B.32)

∂R

∂θz
=


−szcy −cycz 0

−sxsysz + cxcz −sxsycz − szcx 0

sxcz + syszcx −sxsz + sycxcz 0

 (B.33)

∂2R

∂θ2x
=


0 0 0

−sxsycz − szcx sxsysz − cxcz sxcy

−sxsz + sycxcz −sxcz − syszcx −cxcy

 (B.34)

∂2R

∂θ2y
=


−cycz szcy −sy

−sxsycz sxsysz sxcy

sycxcz −syszcx −cxcy

 (B.35)

∂2R

∂θ2z
=


−cycz szcy 0

−sxsycz − szcx sxsysz − cxcz 0

−sxsz + sycxcz −sxcz − syszcx 0

 (B.36)

∂2R

∂θx∂θy
=


0 0 0

cxcycz −szcxcy sycx

sxcycz −sxszcy sxsy

 (B.37)

∂2R

∂θx∂θz
=


0 0 0

−sxcz − syszcx sxsz − sycxcz 0

−sxsysz + cxcz −sxsycz − szcx 0

 (B.38)

∂2R

∂θy∂θz
=


sysz sycz 0

−sxszcy −sxcycz 0

szcxcy cxcycz 0

 (B.39)
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Therefore, we can derive ja,Hab, Za, Zab from eq. (B.31) to eq. (B.39).

jtx = [1, 0, 0]T jty = [0, 1, 0]T jtz = [0, 0, 1]T (B.40)

jθx =
∂R

∂θx
µp jθy =

∂R

∂θy
µp jθz =

∂R

∂θz
µp (B.41)

Hθxθx =
∂2R

∂θ2x
µp Hθyθy =

∂2R

∂θ2y
µp Hθzθz =

∂2R

∂θ2z
µp (B.42)

Hθxθy =
∂2R

∂θxθy
µp Hθxθz =

∂2R

∂θxθz
µp Hθyθz =

∂2R

∂θyθz
µp (B.43)

Note thatHab = 0 when a or b ∈ {tx, ty, tz}.

Ztx = Zty = Ztz = 03×3 (B.44)

Zθx =
∂R

∂θx
ΣpR

T + (
∂R

∂θx
ΣpR

T )T (B.45)

Zθy =
∂R

∂θy
ΣpR

T + (
∂R

∂θy
ΣpR

T )T (B.46)

Zθz =
∂R

∂θz
ΣpR

T + (
∂R

∂θz
ΣpR

T )T (B.47)

Zθxθx = (
∂2R

∂θ2x
ΣpR

T +
∂R

∂θx
Σp(

∂R

∂θx
)T ) + (

∂2R

∂θ2x
ΣpR

T +
∂R

∂θx
Σp(

∂R

∂θx
)T )T (B.48)

Zθyθy = (
∂2R

∂θ2y
ΣpR

T +
∂R

∂θy
Σp(

∂R

∂θy
)T ) + (

∂2R

∂θ2y
ΣpR

T +
∂R

∂θy
Σp(

∂R

∂θy
)T )T (B.49)

Zθzθz = (
∂2R

∂θ2z
ΣpR

T +
∂R

∂θz
Σp(

∂R

∂θz
)T ) + (

∂2R

∂θ2z
ΣpR

T +
∂R

∂θz
Σp(

∂R

∂θz
)T )T (B.50)

Zθxθy = (
∂2R

∂θx∂θy
ΣpR

T +
∂R

∂θx
Σp(

∂R

∂θy
)T ) + (

∂2R

∂θx∂θy
ΣpR

T +
∂R

∂θx
Σp(

∂R

∂θy
)T )T (B.51)

Zθxθz = (
∂2R

∂θx∂θz
ΣpR

T +
∂R

∂θx
Σp(

∂R

∂θz
)T ) + (

∂2R

∂θx∂θz
ΣpR

T +
∂R

∂θx
Σp(

∂R

∂θz
)T )T (B.52)

Zθyθz = (
∂2R

∂θy∂θz
ΣpR

T +
∂R

∂θy
Σp(

∂R

∂θz
)T ) + (

∂2R

∂θy∂θz
ΣpR

T +
∂R

∂θy
Σp(

∂R

∂θz
)T )T (B.53)

Note that Zab = 03×3 when a or b ∈ {tx, ty, tz}.

Finally, the values of eq. (B.24) and eq. (B.26) can be computed.
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